Added Pos/Neg flags, updated Test, changed Soundness lemma slightly

StaticAnalyzer.dfy
@@ -1,59 +1,12 @@
 // ECS 261 Final Project
 // StaticAnalyzer.dfy
 
+include "Types.dfy" 
+
 module StaticAnalyzer {    
-    // AST Syntax Definition
+    import opened Types
 
-    // abstract state of variables, not like the dynamically updated map of variables but is able to track certain aspects of the variables
-    // datatype AbsVal = Zero | NonZero | Unknown
-    datatype AbsVal = Zero | NonZero | Unknown
-    type AbsState = map<string, AbsVal>
-    
-    // Expression datatype
-    datatype Expr =
-        | Const(n: int)
-        | Var(x: string)
-        | Add(e1: Expr, e2: Expr)
-        | Sub(e1: Expr, e2: Expr)
-        | Mul(e1: Expr, e2: Expr)
-        | Div(e1: Expr, e2: Expr)
-        | Mod(e1: Expr, e2: Expr) 
-
-    // Statement datatype
-    datatype Stmt =
-        | Skip
-        | Assign(x: string, e: Expr)
-        | Seq(s1: Stmt, s2: Stmt)
-        | If(cond: Expr, t: Stmt, f: Stmt)
-
-    // Runtime model
-    
-    // We model the concrete environment as a map with variable names as the keys to their corresponding values as the value.
-    // If a variable is missing from the map, it is "uninitialized", and it will cause an error if it accessed (without having been initialized).
-    type Env = map<string, int>
-
-    // Runtime errors to detect for.
-    datatype RuntimeError =
-        | DivByZero
-        | UninitializedVar(x: string)
-        // out of bounds
-
-    // Result can either be Ok, or a runtime error.
-    datatype Result<T> =
-        | Ok(v: T)
-        | Err(e: RuntimeError)
-
-    // Set/Update a variable
-    function Update(env: Env, x: string, v: int): Env
-        ensures x in Update(env, x, v)
-        ensures Update(env, x, v)[x] == v
-    {
-        env[x := v]
-    }
-
-    // -----------------------------
-    // 3) Expression evaluation (runtime)
-    // -----------------------------
+    // Expression evaluation (runtime simulation)
     function EvalExpr(e: Expr, env: Env): Result<int>
         decreases e
     {
@@ -115,6 +68,7 @@ module StaticAnalyzer {
                 }
             }
 
+        // If e is a modulo between two expressions, evaluate the expressions, checking for errors.
         case Mod(a,b) =>
             match EvalExpr(a, env) {
             case Err(er) => Err(er)
@@ -162,45 +116,69 @@ module StaticAnalyzer {
             }
     }
 
+    // Abstract evaluation of an expression
     function AbsEval(e: Expr, state: AbsState): AbsVal        
         decreases e
     {
         match e
-        case Const(n) => if n == 0 then Zero else NonZero
+        // if constant, simply evaluate the constant.
+        case Const(n) => if n == 0 then Zero else if n > 0 then Positive else Negative
 
+        // if variable, check if the variable exists, and use that state.
         case Var(x) => if x in state then state[x] else Unknown
 
+        // for addition check all the valid cases where we can evaluate the abstract value, else unknown
         case Add(a,b) =>
             var a_eval := AbsEval(a, state);
             var b_eval := AbsEval(b, state);
             
             if a_eval == Zero && b_eval == Zero then Zero
-            else if a_eval == NonZero && b_eval == Zero then NonZero
-            else if a_eval == Zero && b_eval == NonZero then NonZero
+            else if a_eval == Positive && b_eval == Zero then Positive
+            else if a_eval == Negative && b_eval == Zero then Negative
+            else if a_eval == Zero && b_eval == Positive then Positive
+            else if a_eval == Zero && b_eval == Negative then Negative
+            else if a_eval == Positive && b_eval == Positive then Positive
+            else if a_eval == Negative && b_eval == Negative then Negative
             else Unknown
 
+        // for subtraction check all the valid cases where we can evaluate the abstract value, else unknown
         case Sub(a,b) =>
             var a_eval := AbsEval(a, state);
             var b_eval := AbsEval(b, state);
             
             if a_eval == Zero && b_eval == Zero then Zero
-            else if a_eval == NonZero && b_eval == Zero then NonZero
-            else if a_eval == Zero && b_eval == NonZero then NonZero
+            else if a_eval == Positive && b_eval == Zero then Positive
+            else if a_eval == Negative && b_eval == Zero then Negative
+            else if a_eval == Zero && b_eval == Positive then Negative
+            else if a_eval == Zero && b_eval == Negative then Positive
+            else if a_eval == Positive && b_eval == Negative then Positive
+            else if a_eval == Negative && b_eval == Positive then Negative
             else Unknown
 
+        // for mult check all the valid cases where we can evaluate the abstract value, else unknown
         case Mul(a,b) =>
             var a_eval := AbsEval(a, state);
             var b_eval := AbsEval(b, state);
 
             if a_eval == Zero || b_eval == Zero then Zero
-            else if a_eval == NonZero && b_eval == NonZero then NonZero
+            else if a_eval == Positive && b_eval == Positive then Positive
+            else if a_eval == Negative && b_eval == Negative then Positive
+            else if a_eval == Positive && b_eval == Negative then Negative
+            else if a_eval == Negative && b_eval == Positive then Negative
             else Unknown
 
+        // for div check all the valid cases where we can evaluate the abstract value, else unknown
         case Div(a, b) => 
-            if AbsEval(a, state) == Zero && AbsEval(b, state) == NonZero then Zero else Unknown
-
+            var a_eval := AbsEval(a, state);
+            var b_eval := AbsEval(b, state);
+            if a_eval == Zero then Zero
+            else Unknown
+        
+        // for mult check all the valid cases where we can evaluate the abstract value, else unknown
         case Mod(a, b) => 
-            if AbsEval(a, state) == Zero && AbsEval(b, state) == NonZero then Zero else Unknown
+            var a_eval := AbsEval(a, state);            
+            if a_eval == Zero then Zero
+            else Unknown
     }
     
     function CheckExpr(e: Expr, state: AbsState): bool
@@ -208,59 +186,79 @@ module StaticAnalyzer {
     {
         match e
 
+        // if constant, then automatically valid
         case Const(n) => true
 
+        // if variable, then check if variable name is in state.
         case Var(x) => x in state
 
+        // if add operation, recursively check both subexp.
         case Add(a,b) => CheckExpr(a, state) && CheckExpr(b, state)
         
+        // if sub operation, recursively check both subexp.
         case Sub(a,b) => CheckExpr(a, state) && CheckExpr(b, state)
         
+        // if mul operation, recursively check both subexp.
         case Mul(a,b) => CheckExpr(a, state) && CheckExpr(b, state)
 
-        case Div(a,b) => CheckExpr(a, state) && CheckExpr(b, state) && AbsEval(b, state) == NonZero
+        // if div operation, recursively check both subexp. additionally check abseval on denom for zero/unknown.
+        case Div(a,b) => CheckExpr(a, state) && CheckExpr(b, state) && (AbsEval(b, state) == Positive || AbsEval(b, state) == Negative)
 
-        case Mod(a,b) => CheckExpr(a, state) && CheckExpr(b, state) && AbsEval(b, state) == NonZero
+        // if mod operation, recursively check both subexp. additionally check abseval on denom for zero/unknown.
+        case Mod(a,b) => CheckExpr(a, state) && CheckExpr(b, state) && (AbsEval(b, state) == Positive || AbsEval(b, state) == Negative)
     }
 
+    // helper for joinstate, combine two absval (if they are unequal, result in unknown)
     function JoinVal(a: AbsVal, b: AbsVal): AbsVal
     {
         if a == b then a else Unknown
     }
 
+    // joins two states (used in analysis of if statements)
     function JoinState(s1: AbsState, s2: AbsState): AbsState
     {
         map k | k in s1 && k in s2 :: JoinVal(s1[k], s2[k])
     }
 
+    // main function for static analyzer.
     function AnalyzeStmt(s: Stmt, state: AbsState): (bool, AbsState)
         decreases s
     {
         match s
 
+        // skip statement will trivially be safe
         case Skip => (true, state)
 
+        // verify the expression e is valid, if so, then safe otherwise not.
         case Assign(x, e) =>
             if CheckExpr(e, state)
             then (true, state[x := AbsEval(e, state)])
             else (false, state)
         
+        // recursively analyze both sub statements.
         case Seq(s1, s2) =>
             match AnalyzeStmt(s1, state){
                 case (false, state_f_s1) => (false, state_f_s1)
                 case (true, state_t_s1) => AnalyzeStmt(s2, state_t_s1)
             }
 
+        // if condition
         case If(cond, then_statement, else_statement) =>
+            // first check the condition expression.
             if(CheckExpr(cond, state))
                 then match AbsEval(cond, state)
-                    case NonZero => AnalyzeStmt(then_statement, state)
+                    // if positive or negative analyze then statement only (pruning)
+                    case Positive => AnalyzeStmt(then_statement, state)
+                    case Negative => AnalyzeStmt(then_statement, state)
+                    // if zero analyze else statement only (pruning)
                     case Zero => AnalyzeStmt(else_statement, state)
+                    // if unknown analyze both statements.
                     case Unknown => match AnalyzeStmt(then_statement, state){
                             case (false, state_f_then) => (false, state_f_then)
                             case (true, state_t_then) =>
                                 match AnalyzeStmt(else_statement, state) {
                                     case (false, state_f_else) => (false, state_f_else)
+                                    // use join statement to take the intersection of both sides.
                                     case (true, state_t_else) => (true, JoinState(state_t_then, state_t_else))
                                 }
                         }
@@ -274,38 +272,45 @@ module StaticAnalyzer {
         case Err(_) => true
     }
 
+    // important invariant: verifies consistency between abstract state and env (used as precondition)
     predicate Consistent(st: AbsState, env: Env){
         forall x :: x in st ==>
             x in env &&
             (st[x] == Zero ==> env[x] == 0) &&
-            (st[x] == NonZero ==> env[x] != 0)
+            (st[x] == Positive ==> env[x] > 0) &&
+            (st[x] == Negative ==> env[x] < 0)
     }
 
-    lemma AbsNonZeroOkValueNonZero(e: Expr, st: AbsState, env: Env, v: int)
-        requires AbsEval(e, st) == NonZero
+    // lemma: if absstate indicates positive, then the env will have a positive value for the variable at that state.
+    lemma {:vcs_split_on_every_assert} AbsPositiveOkValuePositive(e: Expr, st: AbsState, env: Env, v: int)
+        requires AbsEval(e, st) == Positive
         requires CheckExpr(e, st)
         requires Consistent(st, env)
         requires EvalExpr(e, env) == Ok(v)
-        ensures v != 0
+        ensures v > 0
         decreases e
     {
         match e
         
+        // if constant, simply check the value if positive.
         case Const(n) => {
-            assert n != 0;
+            assert n > 0;
             assert v == n;
         }
 
-        case Var(n) => {
-            assert n in st && n in env;
-            assert env[n] != 0;
+        // if variable, the variable must exist and value must match as well.
+        case Var(x) => {
+            assert x in st && x in env;
+            assert st[x] == Positive;
+            assert env[x] > 0;
+            assert v == env[x];
         }
 
-        case Add(a, b) => {
-            var a_eval := AbsEval(a, st);
-            var b_eval := AbsEval(b, st);
-
-            assert (a_eval == NonZero && b_eval == Zero) || (a_eval == Zero && b_eval == NonZero);
+        // if add then verify expression evaluates to positive
+        case Add(a,b) => {
+            var va := AbsEval(a, st);
+            var vb := AbsEval(b, st);
+            assert (va == Positive && vb == Zero) || (va == Zero && vb == Positive) || (va == Positive && vb == Positive);
 
             CheckTrueEvalValid(a, st, env);
             CheckTrueEvalValid(b, st, env);
@@ -315,26 +320,34 @@ module StaticAnalyzer {
                 match EvalExpr(b, env)
                 case Ok(v2) => {
                     assert v == v1 + v2;
-                    if(a_eval == NonZero){
-                        AbsZeroOkValueZero(b, st, env, v2);
-                        AbsNonZeroOkValueNonZero(a, st, env, v1);
-                        assert v2 == 0;
-                    } else{
+                    // assert each of the cases, positive can be possible.
+                    if va == Zero {
                         AbsZeroOkValueZero(a, st, env, v1);
-                        AbsNonZeroOkValueNonZero(b, st, env, v2);
+                        AbsPositiveOkValuePositive(b, st, env, v2);
                         assert v1 == 0;
+                        assert v2 > 0;
+                    } else if vb == Zero {
+                        AbsPositiveOkValuePositive(a, st, env, v1);
+                        AbsZeroOkValueZero(b, st, env, v2);
+                        assert v1 > 0;
+                        assert v2 == 0;
+                    } else {
+                        AbsPositiveOkValuePositive(a, st, env, v1);
+                        AbsPositiveOkValuePositive(b, st, env, v2);
+                        assert v1 > 0 && v2 > 0;
                     }
+                    assert v > 0;
                 }
                 case Err(_) => assert false;
             }
             case Err(_) => assert false;
         }
 
-        case Sub(a, b) => {
-            var a_eval := AbsEval(a, st);
-            var b_eval := AbsEval(b, st);
-
-            assert (a_eval == NonZero && b_eval == Zero) || (a_eval == Zero && b_eval == NonZero);
+        // sub case, similar to add case
+        case Sub(a,b) => {
+            var va := AbsEval(a, st);
+            var vb := AbsEval(b, st);
+            assert (va == Positive && vb == Zero) || (va == Zero && vb == Negative) || (va == Positive && vb == Negative);
 
             CheckTrueEvalValid(a, st, env);
             CheckTrueEvalValid(b, st, env);
@@ -344,14 +357,254 @@ module StaticAnalyzer {
                 match EvalExpr(b, env)
                 case Ok(v2) => {
                     assert v == v1 - v2;
-                    if(a_eval == NonZero){
+                    if va == Positive && vb == Zero {
+                        AbsPositiveOkValuePositive(a, st, env, v1);
                         AbsZeroOkValueZero(b, st, env, v2);
-                        AbsNonZeroOkValueNonZero(a, st, env, v1);
+                        assert v1 > 0 && v2 == 0;
+                    } else if va == Zero && vb == Negative {
+                        AbsZeroOkValueZero(a, st, env, v1);
+                        AbsNegativeOkValueNegative(b, st, env, v2);
+                        assert v1 == 0 && v2 < 0;
+                    } else {
+                        AbsPositiveOkValuePositive(a, st, env, v1);
+                        AbsNegativeOkValueNegative(b, st, env, v2);
+                        assert v1 > 0 && v2 < 0;
+                    }
+                    assert v > 0;
+                }
+                case Err(_) => assert false;
+            }
+            case Err(_) => assert false;
+        }
+
+        // mul case, similar to add case
+        case Mul(a,b) => {
+            var va := AbsEval(a, st);
+            var vb := AbsEval(b, st);
+            assert (va == Positive && vb == Positive) || (va == Negative && vb == Negative);
+
+            CheckTrueEvalValid(a, st, env);
+            CheckTrueEvalValid(b, st, env);
+
+            match EvalExpr(a, env)
+            case Ok(v1) => {
+                match EvalExpr(b, env)
+                case Ok(v2) => {
+                    assert v == v1 * v2;
+                    if va == Positive {
+                        AbsPositiveOkValuePositive(a, st, env, v1);
+                        AbsPositiveOkValuePositive(b, st, env, v2);
+                        assert v1 > 0 && v2 > 0;
+                    } else {
+                        AbsNegativeOkValueNegative(a, st, env, v1);
+                        AbsNegativeOkValueNegative(b, st, env, v2);
+                        assert v1 < 0 && v2 < 0;
+                    }
+                    assert v > 0;
+                }
+                case Err(_) => assert false;
+            }
+            case Err(_) => assert false;
+        }
+
+        // div case, since you can never fully assert a positive (non-zero) result from module, given my language syntax, it's impossible.
+        case Div(a,b) => assert false;
+
+        // mod case, since you can never fully assert a positive (non-zero) result from module, given my language syntax, it's impossible.
+        case Mod(a,b) => assert false;
+    }
+
+    // lemma: if absstate indicates negative, then the env will have a negative value for the variable at that state.
+    lemma {:vcs_split_on_every_assert} AbsNegativeOkValueNegative(e: Expr, st: AbsState, env: Env, v: int)
+        requires AbsEval(e, st) == Negative
+        requires CheckExpr(e, st)
+        requires Consistent(st, env)
+        requires EvalExpr(e, env) == Ok(v)
+        ensures v < 0
+        decreases e
+    {
+        match e
+        // constant case, verify that constant is negative
+        case Const(n) => {
+            assert n < 0;
+            assert v == n;
+        }
+
+        // variable case, assert the variable exists in both state and env and that the val is negative 
+        case Var(x) => {
+            assert x in st && x in env;
+            assert st[x] == Negative;
+            assert env[x] < 0;
+            assert v == env[x];
+        }
+
+        // add case 
+        case Add(a,b) => {
+            var va := AbsEval(a, st);
+            var vb := AbsEval(b, st);
+            assert (va == Negative && vb == Zero) || (va == Zero && vb == Negative) || (va == Negative && vb == Negative);
+            CheckTrueEvalValid(a, st, env);
+            CheckTrueEvalValid(b, st, env);
+
+            // assert each of the cases, negative can be possible.
+            match EvalExpr(a, env)
+            case Ok(v1) => {
+                match EvalExpr(b, env)
+                case Ok(v2) => {
+                    assert v == v1 + v2;
+                    if va == Zero {
+                        AbsZeroOkValueZero(a, st, env, v1);
+                        AbsNegativeOkValueNegative(b, st, env, v2);
+                        assert v1 == 0;
+                        assert v2 < 0;
+                    } else if vb == Zero {
+                        AbsNegativeOkValueNegative(a, st, env, v1);
+                        AbsZeroOkValueZero(b, st, env, v2);
+                        assert v1 < 0;
                         assert v2 == 0;
-                    } else{
+                    } else {
+                        AbsNegativeOkValueNegative(a, st, env, v1);
+                        AbsNegativeOkValueNegative(b, st, env, v2);
+                        assert v1 < 0 && v2 < 0;
+                    }
+                    assert v < 0;
+                }
+                case Err(_) => assert false;
+            }
+            case Err(_) => assert false;
+        }
+
+        // sub case
+        case Sub(a,b) => {
+            var va := AbsEval(a, st);
+            var vb := AbsEval(b, st);
+            assert (va == Negative && vb == Zero) || (va == Zero && vb == Positive) || (va == Negative && vb == Positive);
+
+            CheckTrueEvalValid(a, st, env);
+            CheckTrueEvalValid(b, st, env);
+
+            match EvalExpr(a, env)
+            case Ok(v1) => {
+                match EvalExpr(b, env)
+                case Ok(v2) => {
+                    assert v == v1 - v2;
+                    if va == Negative && vb == Zero {
+                        AbsNegativeOkValueNegative(a, st, env, v1);
+                        AbsZeroOkValueZero(b, st, env, v2);
+                        assert v1 < 0 && v2 == 0;
+                    } else if va == Zero && vb == Positive {
+                        AbsZeroOkValueZero(a, st, env, v1);
+                        AbsPositiveOkValuePositive(b, st, env, v2);
+                        assert v1 == 0 && v2 > 0;
+                    } else {
+                        AbsNegativeOkValueNegative(a, st, env, v1);
+                        AbsPositiveOkValuePositive(b, st, env, v2);
+                        assert v1 < 0 && v2 > 0;
+                    }
+                    assert v < 0;
+                }
+                case Err(_) => assert false;
+            }
+            case Err(_) => assert false;
+        }
+
+        // mul case
+        case Mul(a,b) => {
+            var va := AbsEval(a, st);
+            var vb := AbsEval(b, st);
+            assert (va == Positive && vb == Negative) || (va == Negative && vb == Positive);
+
+            CheckTrueEvalValid(a, st, env);
+            CheckTrueEvalValid(b, st, env);
+
+            match EvalExpr(a, env)
+            case Ok(v1) => {
+                match EvalExpr(b, env)
+                case Ok(v2) => {
+                    assert v == v1 * v2;
+                    if va == Positive {
+                        AbsPositiveOkValuePositive(a, st, env, v1);
+                        AbsNegativeOkValueNegative(b, st, env, v2);
+                        assert v1 > 0 && v2 < 0;
+                    } else {
+                        AbsNegativeOkValueNegative(a, st, env, v1);
+                        AbsPositiveOkValuePositive(b, st, env, v2);
+                        assert v1 < 0 && v2 > 0;
+                    }
+                    assert v < 0;
+                }
+                case Err(_) => assert false;
+            }
+            case Err(_) => assert false;
+        }
+
+        // div case
+        case Div(a,b) => assert false;
+
+        // mod never results in negative
+        case Mod(a,b) => assert false;
+    }
+
+    lemma {:vcs_split_on_every_assert} AbsNonZeroOkValueNonZero(e: Expr, st: AbsState, env: Env, v: int)
+        requires (AbsEval(e, st) == Positive || AbsEval(e, st) == Negative) 
+        requires CheckExpr(e, st)
+        requires Consistent(st, env)
+        requires EvalExpr(e, env) == Ok(v)
+        ensures v != 0
+        decreases e
+    {
+        match e
+
+        // constant case: assert that the value is NonZero
+        case Const(n) => {
+            assert n != 0;
+            assert v == n;
+        }
+
+        // variable case: assert that the value exists and it's NonZero
+        case Var(x) => {
+            assert x in st && x in env;
+            if st[x] == Positive {
+                assert env[x] > 0;
+            } else {
+                assert st[x] == Negative;
+                assert env[x] < 0;
+            }
+            assert v == env[x];
+        }
+
+        // add case, cover all potential add combinations as defined in AbsEval
+        case Add(a,b) => {
+            var va := AbsEval(a, st);
+            var vb := AbsEval(b, st);
+            assert (va == Positive && vb == Zero) || (va == Zero && vb == Positive) ||
+                   (va == Negative && vb == Zero) || (va == Zero && vb == Negative) ||
+                   (va == Positive && vb == Positive) || (va == Negative && vb == Negative);
+
+            CheckTrueEvalValid(a, st, env);
+            CheckTrueEvalValid(b, st, env);
+
+            match EvalExpr(a, env)
+            case Ok(v1) => {
+                match EvalExpr(b, env)
+                case Ok(v2) => {
+                    assert v == v1 + v2;
+                    if va == Zero {
                         AbsZeroOkValueZero(a, st, env, v1);
                         AbsNonZeroOkValueNonZero(b, st, env, v2);
                         assert v1 == 0;
+                    } else if vb == Zero {
+                        AbsNonZeroOkValueNonZero(a, st, env, v1);
+                        AbsZeroOkValueZero(b, st, env, v2);
+                        assert v2 == 0;
+                    } else if va == Positive {
+                        AbsPositiveOkValuePositive(a, st, env, v1);
+                        AbsPositiveOkValuePositive(b, st, env, v2);
+                        assert v1 > 0 && v2 > 0;
+                    } else {
+                        AbsNegativeOkValueNegative(a, st, env, v1);
+                        AbsNegativeOkValueNegative(b, st, env, v2);
+                        assert v1 < 0 && v2 < 0;
                     }
                 }
                 case Err(_) => assert false;
@@ -359,11 +612,57 @@ module StaticAnalyzer {
             case Err(_) => assert false;
         }
 
-        case Mul(a, b) => {
-            var a_eval := AbsEval(a, st);
-            var b_eval := AbsEval(b, st);
+        // sub case, same as add more or less
+        case Sub(a,b) => {
+            var va := AbsEval(a, st);
+            var vb := AbsEval(b, st);
+            assert (va == Positive && vb == Zero) || (va == Zero && vb == Negative) || (va == Positive && vb == Negative) ||
+                   (va == Negative && vb == Zero) || (va == Zero && vb == Positive) || (va == Negative && vb == Positive);
 
-            assert (a_eval == NonZero && b_eval == NonZero);
+            CheckTrueEvalValid(a, st, env);
+            CheckTrueEvalValid(b, st, env);
+
+            match EvalExpr(a, env)
+            case Ok(v1) => {
+                match EvalExpr(b, env)
+                case Ok(v2) => {
+                    assert v == v1 - v2;
+                    if va == Positive && vb == Zero {
+                        AbsPositiveOkValuePositive(a, st, env, v1);
+                        AbsZeroOkValueZero(b, st, env, v2);
+                        assert v1 > 0;
+                    } else if va == Zero && vb == Negative {
+                        AbsZeroOkValueZero(a, st, env, v1);
+                        AbsNegativeOkValueNegative(b, st, env, v2);
+                        assert v2 < 0;
+                    } else if va == Positive && vb == Negative {
+                        AbsPositiveOkValuePositive(a, st, env, v1);
+                        AbsNegativeOkValueNegative(b, st, env, v2);
+                    } else if va == Negative && vb == Zero {
+                        AbsNegativeOkValueNegative(a, st, env, v1);
+                        AbsZeroOkValueZero(b, st, env, v2);
+                        assert v1 < 0;
+                    } else if va == Zero && vb == Positive {
+                        AbsZeroOkValueZero(a, st, env, v1);
+                        AbsPositiveOkValuePositive(b, st, env, v2);
+                        assert v2 > 0;
+                    } else {
+                        AbsNegativeOkValueNegative(a, st, env, v1);
+                        AbsPositiveOkValuePositive(b, st, env, v2);
+                    }
+                    assert v != 0;
+                }
+                case Err(_) => assert false;
+            }
+            case Err(_) => assert false;
+        }
+
+        // mul case, same as add more or less
+        case Mul(a,b) => {
+            var va := AbsEval(a, st);
+            var vb := AbsEval(b, st);
+            assert (va == Positive && vb == Positive) || (va == Negative && vb == Negative) ||
+                   (va == Positive && vb == Negative) || (va == Negative && vb == Positive);
 
             CheckTrueEvalValid(a, st, env);
             CheckTrueEvalValid(b, st, env);
@@ -382,13 +681,15 @@ module StaticAnalyzer {
             case Err(_) => assert false;
         }
 
-        case Div(a, b) => assert false;
+        //div case, mod cannot be asserted to be nonzero in any case.
+        case Div(a,b) => assert false;
 
-        case Mod(a, b) => assert false;
+        //mod case, mod cannot be asserted to be nonzero in any case.
+        case Mod(a,b) => assert false;
     }
 
     // If AbsEval says "Zero", then any Ok(v) must be v == 0
-    lemma AbsZeroOkValueZero(e: Expr, st: AbsState, env: Env, v: int)
+    lemma {:vcs_split_on_every_assert} AbsZeroOkValueZero(e: Expr, st: AbsState, env: Env, v: int)
         requires AbsEval(e, st) == Zero
         requires CheckExpr(e, st)
         requires Consistent(st, env)
@@ -397,11 +698,13 @@ module StaticAnalyzer {
         decreases e
     {
         match e
+        // assert if exp is a const and abseval gives 0, then the constant value is 0.
         case Const(n) => {
             assert n == 0;
             assert v == 0;
         }
 
+        // var case: assert that the item exists in state and env, and that it equals 0.
         case Var(x) => {
             assert x in st;
             assert x in env;
@@ -410,6 +713,7 @@ module StaticAnalyzer {
             assert v == env[x];
         }
 
+        // add case: go through each possibility for add, and assert every case to be working towards resulting in 0.
         case Add(a,b) => {
             CheckTrueEvalValid(a, st, env);
             CheckTrueEvalValid(b, st, env);
@@ -428,6 +732,7 @@ module StaticAnalyzer {
             case Err(_) => assert false;
         }
 
+        // sub case: same as add more or less
         case Sub(a,b) => {
             CheckTrueEvalValid(a, st, env);
             CheckTrueEvalValid(b, st, env);
@@ -446,6 +751,7 @@ module StaticAnalyzer {
             case Err(_) => assert false;
         }
 
+        // mul case: same as add more or less
         case Mul(a,b) => {
             var va := AbsEval(a, st);
             var vb := AbsEval(b, st);
@@ -472,9 +778,9 @@ module StaticAnalyzer {
             case Err(_) => assert false;
         }
 
+        // div case: same as add more or less
         case Div(a,b) => {
-            assert AbsEval(a, st) == Zero && AbsEval(b, st) == NonZero;
-
+            assert AbsEval(a, st) == Zero && (AbsEval(b, st) == Positive || AbsEval(b, st) == Negative);
             CheckTrueEvalValid(a, st, env);
             CheckTrueEvalValid(b, st, env);
 
@@ -493,8 +799,9 @@ module StaticAnalyzer {
             case Err(_) => assert false;
         }
 
+        // mod case: same as add more or less
         case Mod(a,b) => {
-            assert AbsEval(a, st) == Zero && AbsEval(b, st) == NonZero;
+            assert AbsEval(a, st) == Zero && (AbsEval(b, st) == Positive || AbsEval(b, st) == Negative);
 
             CheckTrueEvalValid(a, st, env);
             CheckTrueEvalValid(b, st, env);
@@ -515,6 +822,8 @@ module StaticAnalyzer {
         }
     }
 
+    // this lemma asserts that if checkexpr indicates a given expression is safe
+    // then that expression will not result in an error when evaluated.
     lemma CheckTrueEvalValid(e: Expr, st: AbsState, env: Env)
         requires CheckExpr(e, st)
         requires Consistent(st, env)
@@ -522,75 +831,91 @@ module StaticAnalyzer {
         decreases e
     {
         match e
+        // trivial: if we have a constant, we simply can assert that the result is as expected.
         case Const(n) => {
             assert EvalExpr(Const(n), env) == Ok(n);
         }
 
+        // we can assert that x exists in both st and env due to check expr and consistency precond's
         case Var(x) => {
             assert x in st;
-            assert x in env; // from Consistent
+            assert x in env;
+            // we can assert that the values will be same as well on evaluation
             assert EvalExpr(Var(x), env) == Ok(env[x]);
         }
 
+        // add case
         case Add(a,b) => {
+            //assert that both subexpressions are safe, and eval are valid (recursive calls)
             assert CheckExpr(a, st) && CheckExpr(b, st);
             CheckTrueEvalValid(a, st, env);
             CheckTrueEvalValid(b, st, env);
 
-            match EvalExpr(a, env)
-            case Ok(v1) => {
-            match EvalExpr(b, env)
-            case Ok(v2) => {
-                assert EvalExpr(Add(a,b), env) == Ok(v1 + v2);
-            }
-            case Err(_) => assert false;
-            }
-            case Err(_) => assert false;
-        }
-
-        case Sub(a,b) => {
-            assert CheckExpr(a, st) && CheckExpr(b, st);
-            CheckTrueEvalValid(a, st, env);
-            CheckTrueEvalValid(b, st, env);
-
-            match EvalExpr(a, env)
-            case Ok(v1) => {
-            match EvalExpr(b, env)
-            case Ok(v2) => {
-                assert EvalExpr(Sub(a,b), env) == Ok(v1 - v2);
-            }
-            case Err(_) => assert false;
-            }
-            case Err(_) => assert false;
-        }
-
-        case Mul(a,b) => {
-            assert CheckExpr(a, st) && CheckExpr(b, st);
-            CheckTrueEvalValid(a, st, env);
-            CheckTrueEvalValid(b, st, env);
-
-            match EvalExpr(a, env)
-            case Ok(v1) => {
-            match EvalExpr(b, env)
-            case Ok(v2) => {
-                assert EvalExpr(Mul(a,b), env) == Ok(v1 * v2);
-            }
-            case Err(_) => assert false;
-            }
-            case Err(_) => assert false;
-        }
-
-        case Div(a,b) => {
-            assert CheckExpr(a, st) && CheckExpr(b, st);
-            assert AbsEval(b, st) == NonZero;
-
-            CheckTrueEvalValid(a, st, env);
-            CheckTrueEvalValid(b, st, env);
-
+            // assert that the expected results result in the sum of the two values.
             match EvalExpr(a, env)
             case Ok(v1) => {
                 match EvalExpr(b, env)
                 case Ok(v2) => {
+                    assert EvalExpr(Add(a,b), env) == Ok(v1 + v2);
+                }
+                case Err(_) => assert false;
+            }
+            case Err(_) => assert false;
+        }
+
+        // sub case
+        case Sub(a,b) => {
+            //assert that both subexpressions are safe, and eval are valid (recursive calls)
+            assert CheckExpr(a, st) && CheckExpr(b, st);
+            CheckTrueEvalValid(a, st, env);
+            CheckTrueEvalValid(b, st, env);
+
+            // assert that the expected results result in the difference of the two values.
+            match EvalExpr(a, env)
+            case Ok(v1) => {
+                match EvalExpr(b, env)
+                case Ok(v2) => {
+                    assert EvalExpr(Sub(a,b), env) == Ok(v1 - v2);
+                }
+                case Err(_) => assert false;
+            }
+            case Err(_) => assert false;
+        }
+
+        // mul case
+        case Mul(a,b) => {
+            //assert that both subexpressions are safe, and eval are valid (recursive calls)
+            assert CheckExpr(a, st) && CheckExpr(b, st);
+            CheckTrueEvalValid(a, st, env);
+            CheckTrueEvalValid(b, st, env);
+
+            // assert that the expected results result in the product of the two values.
+            match EvalExpr(a, env)
+            case Ok(v1) => {
+                match EvalExpr(b, env)
+                case Ok(v2) => {
+                    assert EvalExpr(Mul(a,b), env) == Ok(v1 * v2);
+                }
+                case Err(_) => assert false;
+            }
+            case Err(_) => assert false;
+        }
+
+        // div case
+        case Div(a,b) => {
+            //assert that both subexpressions are safe, and eval are valid (recursive calls)
+            assert CheckExpr(a, st) && CheckExpr(b, st);
+            CheckTrueEvalValid(a, st, env);
+            CheckTrueEvalValid(b, st, env);
+            // additional assert for denom
+            assert AbsEval(b, st) == Positive || AbsEval(b, st) == Negative;
+
+            // assert that the expected results result in the quotient of the two values.
+            match EvalExpr(a, env)
+            case Ok(v1) => {
+                match EvalExpr(b, env)
+                case Ok(v2) => {
+                    // use helper lemma (if abstate indicates nonzero denom (i.e. pos || neg), then the value in env is nonzero as well.)
                     AbsNonZeroOkValueNonZero(b, st, env, v2);
                     assert v2 != 0;
                     assert EvalExpr(Div(a,b), env) == Ok(v1 / v2);
@@ -600,12 +925,12 @@ module StaticAnalyzer {
             case Err(_) => assert false;
         }
 
+        // mod case, similar in structure to div case.
         case Mod(a,b) => {
             assert CheckExpr(a, st) && CheckExpr(b, st);
-            assert AbsEval(b, st) == NonZero;
-
             CheckTrueEvalValid(a, st, env);
             CheckTrueEvalValid(b, st, env);
+            assert AbsEval(b, st) == Positive || AbsEval(b, st) == Negative;
 
             match EvalExpr(a, env)
             case Ok(v1) => {
@@ -621,6 +946,8 @@ module StaticAnalyzer {
         }
     }
 
+    // this lemma is used for the case when an if cond evaluates to Unknown, and we need to maintain the consistency inv
+    // if the runtime env travels down the then path, its absstate will match the join path's absstate.
     lemma ConsistentJoinLeft(stT: AbsState, stF: AbsState, env: Env)
         requires Consistent(stT, env)
         ensures Consistent(JoinState(stT, stF), env)
@@ -628,25 +955,29 @@ module StaticAnalyzer {
         forall k | k in JoinState(stT, stF)
             ensures k in env
             ensures (JoinState(stT, stF)[k] == Zero ==> env[k] == 0)
-            ensures (JoinState(stT, stF)[k] == NonZero ==> env[k] != 0)
+            ensures (JoinState(stT, stF)[k] == Positive ==> env[k] > 0)
+            ensures (JoinState(stT, stF)[k] == Negative ==> env[k] < 0)
         {
-            // From membership in JoinState:
             assert k in stT && k in stF;
-            assert k in env; // from Consistent(stT, env)
+            assert k in env;
 
-            // JoinState[k] = JoinVal(stT[k], stF[k])
             if JoinState(stT, stF)[k] == Zero {
-            // then JoinVal(...) == Zero, so stT[k] == stF[k] == Zero
-            assert stT[k] == Zero;
-            assert env[k] == 0;
+                assert stT[k] == Zero;
+                assert env[k] == 0;
             }
-            if JoinState(stT, stF)[k] == NonZero {
-            assert stT[k] == NonZero;
-            assert env[k] != 0;
+            if JoinState(stT, stF)[k] == Positive {
+                assert stT[k] == Positive;
+                assert env[k] > 0;
+            }
+            if JoinState(stT, stF)[k] == Negative {
+                assert stT[k] == Negative;
+                assert env[k] < 0;
             }
         }
     }
 
+    // this lemma is used for the case when an if cond evaluates to Unknown, and we need to maintain the consistency inv
+    // if the runtime env travels down the else path, its absstate will match the join path's absstate.
     lemma ConsistentJoinRight(stT: AbsState, stF: AbsState, env: Env)
         requires Consistent(stF, env)
         ensures Consistent(JoinState(stT, stF), env)
@@ -654,22 +985,28 @@ module StaticAnalyzer {
         forall k | k in JoinState(stT, stF)
             ensures k in env
             ensures (JoinState(stT, stF)[k] == Zero ==> env[k] == 0)
-            ensures (JoinState(stT, stF)[k] == NonZero ==> env[k] != 0)
+            ensures (JoinState(stT, stF)[k] == Positive ==> env[k] > 0)
+            ensures (JoinState(stT, stF)[k] == Negative ==> env[k] < 0)
         {
             assert k in stT && k in stF;
-            assert k in env; // from Consistent(stF, env)
+            assert k in env;
 
             if JoinState(stT, stF)[k] == Zero {
-            assert stF[k] == Zero;
-            assert env[k] == 0;
+                assert stF[k] == Zero;
+                assert env[k] == 0;
             }
-            if JoinState(stT, stF)[k] == NonZero {
-            assert stF[k] == NonZero;
-            assert env[k] != 0;
+            if JoinState(stT, stF)[k] == Positive {
+                assert stF[k] == Positive;
+                assert env[k] > 0;
+            }
+            if JoinState(stT, stF)[k] == Negative {
+                assert stF[k] == Negative;
+                assert env[k] < 0;
             }
         }
     }
     
+    // key lemma: essentially if analyzestmt returns true, then execstmt will not result in an error (soundness)
     lemma AnalyzeTrueExecValid(s: Stmt, st: AbsState, env: Env)
         requires AnalyzeStmt(s, st).0
         requires Consistent(st, env)
@@ -681,29 +1018,36 @@ module StaticAnalyzer {
     {
         match s
 
+        // skip case: trivial simply assert no issue will happen.
         case Skip() => assert ExecStmt(Skip(), env) == Ok(env);
 
+        // assign case: 
         case Assign(x, e) => {
+            // check the the expression itself.
             assert CheckExpr(e, st);
             CheckTrueEvalValid(e, st, env);
 
             match EvalExpr(e, env)
             case Ok(v) => {
+                // update the environment (simulating the behavior of Assign itself)
                 var update_env := Update(env, x, v);
+                // prove the soundness implication 
                 assert ExecStmt(Assign(x, e), env) == Ok(update_env);
-
                 var stOut := AnalyzeStmt(Assign(x, e), st).1;
-
                 assert stOut == st[x := AbsEval(e, st)];
-
+                
+                // assert the consistency postcondition.
                 assert Consistent(stOut, update_env) by 
                 {
+                    // loop through each item in output state and check if it's consistent.
                     forall y | y in stOut
                         ensures y in update_env
                         ensures (stOut[y] == Zero ==> update_env[y] == 0)
-                        ensures (stOut[y] == NonZero ==> update_env[y] != 0)
+                        ensures (stOut[y] == Positive ==> update_env[y] > 0)
+                        ensures (stOut[y] == Negative ==> update_env[y] < 0)
                     {
                         if y == x {
+                            // assert that the new element has correctly been added
                             assert y in update_env;
 
                             assert update_env[x] == v;
@@ -716,12 +1060,19 @@ module StaticAnalyzer {
                                 assert update_env[x] == 0;
                             }
 
-                            if stOut[x] == NonZero {
-                                assert AbsEval(e, st) == NonZero;
-                                AbsNonZeroOkValueNonZero(e, st, env, v);
-                                assert update_env[x] != 0;
+                            if stOut[x] == Positive {
+                                assert AbsEval(e, st) == Positive;
+                                AbsPositiveOkValuePositive(e, st, env, v);
+                                assert update_env[x] > 0;
+                            }
+
+                            if stOut[x] == Negative {
+                                assert AbsEval(e, st) == Negative;
+                                AbsNegativeOkValueNegative(e, st, env, v);
+                                assert update_env[x] < 0;
                             }
                         } else {
+                            // assert all old elements are here.
                             assert stOut[y] == st[y];
                             assert y in st && y in env && y in update_env;
 
@@ -733,10 +1084,16 @@ module StaticAnalyzer {
                                 assert update_env[y] == 0;
                             }
 
-                            if stOut[y] == NonZero {
-                                assert st[y] == NonZero;
+                            if stOut[y] == Positive {
+                                assert st[y] == Positive;
                                 assert env[y] != 0;
-                                assert update_env[y] != 0;
+                                assert update_env[y] > 0;
+                            }
+
+                            if stOut[y] == Negative {
+                                assert st[y] == Negative;
+                                assert env[y] != 0;
+                                assert update_env[y] < 0;
                             }
                         }
                     }
@@ -745,33 +1102,36 @@ module StaticAnalyzer {
             case Err(_) => assert false;
         }
 
+        // sequence case: (tricky to maintain consistency btwn two statements (done with invariant))
         case Seq(s1, s2) => {
             var r1 := AnalyzeStmt(s1, st);
+            // show that s1 on it's own is correct w/ recurisve call
             AnalyzeTrueExecValid(s1, st, env);
-
+            
             match ExecStmt(s1, env)
             case Ok(env1) => {
-                // From recursive ensures:
+                // show the abs state from analyzing s1 and the env from execution is consistent
                 assert Consistent(r1.1, env1);
-
+                // show that s2 on it's own is correct w/ recurisve call
                 AnalyzeTrueExecValid(s2, r1.1, env1);
-
-                // ExecStmt(Seq) definition:
+                // we can assert no error from this case.
                 assert !IsErr(ExecStmt(Seq(s1, s2), env));
-                // And output consistency comes from second recursive call
             }
-            case Err(_) => assert false; // impossible by recursive soundness
+            case Err(_) => assert false;
         }
 
+        // if case: 
         case If(cond, t, f) => {
+            // assert that the cond expression is valid and then evaluate it (using abseval)
             assert CheckExpr(cond, st);
             CheckTrueEvalValid(cond, st, env);
-
             var absCond := AbsEval(cond, st);
 
+            // ensure that the abseval dictates the correct direction and that all three potential paths are validated and consistent.
             match EvalExpr(cond, env)
             case Ok(vc) => {
                 match absCond
+                // if zero, only need to look down else path
                 case Zero => {
                     assert AnalyzeStmt(If(cond, t, f), st).1 == AnalyzeStmt(f, st).1;
 
@@ -791,7 +1151,8 @@ module StaticAnalyzer {
                     }
                     case Err(_) => assert false;
                 }
-                case NonZero => {
+                // if positive/negative, only need to look down else path (wrote twice for thoroughness, though code in each case is identical)
+                case Positive => {
                     assert AnalyzeStmt(If(cond, t, f), st).1 == AnalyzeStmt(t, st).1;
 
                     AbsNonZeroOkValueNonZero(cond, st, env, vc);
@@ -810,6 +1171,26 @@ module StaticAnalyzer {
                     }
                     case Err(_) => assert false;
                 }
+                case Negative => {
+                    assert AnalyzeStmt(If(cond, t, f), st).1 == AnalyzeStmt(t, st).1;
+
+                    AbsNonZeroOkValueNonZero(cond, st, env, vc);
+                    assert vc != 0;
+
+                    assert AnalyzeStmt(t, st).0;
+                    AnalyzeTrueExecValid(t, st, env);
+
+                    assert ExecStmt(If(cond, t, f), env) == ExecStmt(t, env);
+                    assert !IsErr(ExecStmt(t, env));
+
+                    match ExecStmt(t, env)
+                    case Ok(envOut) => {
+                        assert Consistent(AnalyzeStmt(t, st).1, envOut);
+                        assert Consistent(AnalyzeStmt(If(cond, t, f), st).1, envOut);
+                    }
+                    case Err(_) => assert false;
+                }
+                // if unknown, we need to use join state to take the intersection.
                 case Unknown => {
                     assert AnalyzeStmt(t, st).0;
                     assert AnalyzeStmt(f, st).0;
@@ -848,28 +1229,25 @@ module StaticAnalyzer {
         }
     }
 
+    // initialize abs state if given a non-empty env to start.
     function AbsInit(env: Env): AbsState
     {
-        map x | x in env ::
-            if env[x] == 0 then Zero else NonZero
+        map x | x in env :: Unknown // if env[x] == 0 then Zero else if env[x] > 0 then Positive else Negative
     }
 
-    lemma AnalyzeProgramInput(p: Stmt, env: Env)
-        requires AnalyzeStmt(p, AbsInit(env)).0
-        ensures !IsErr(ExecStmt(p, env))
+    // wrapper function for analyze statement to extract the result (safe/unsafe).
+    function AnalyzeProgram(p: Stmt, env: Env): bool
     {
-        AnalyzeTrueExecValid(p, AbsInit(env), env);
+        AnalyzeStmt(p, AbsInit(env)).0
     }
 
-    lemma AnalyzeProgramSound(p: Stmt)
-        requires AnalyzeProg(p)
-        ensures !IsErr(ExecStmt(p, map[]))
+    // main soundness lemma: If AnalyzeProgram indicates safe for a program (precond)
+    // then we will not have an error when executing the program. (postcond)
+    lemma AnalyzeProgramSound(p: Stmt, env: Env)
+        ensures AnalyzeProgram(p, env) ==> !IsErr(ExecStmt(p, env))
     {
-        AnalyzeTrueExecValid(p, map[], map[]);
-    }
-
-    function AnalyzeProg(p: Stmt): bool
-    {
-        AnalyzeStmt(p, map[]).0
+        if AnalyzeProgram(p, env){ 
+            AnalyzeTrueExecValid(p, AbsInit(env), env);
+        }
     }
 }
