Types.dfy
@@ -1,0 +1,52 @@
+// ECS 261 Final Project
+// Types.dfy
+
+module Types{
+    // AST Syntax Definition
+
+    // abstract state of variables, not like the dynamically updated map of variables but is able to track certain aspects of the variables
+    datatype AbsVal = Zero | Positive | Negative | Unknown
+    type AbsState = map<string, AbsVal>
+    
+    // Expression datatype
+    datatype Expr =
+        | Const(n: int)
+        | Var(x: string)
+        | Add(e1: Expr, e2: Expr)
+        | Sub(e1: Expr, e2: Expr)
+        | Mul(e1: Expr, e2: Expr)
+        | Div(e1: Expr, e2: Expr)
+        | Mod(e1: Expr, e2: Expr) 
+
+    // Statement datatype
+    datatype Stmt =
+        | Skip
+        | Assign(x: string, e: Expr)
+        | Seq(s1: Stmt, s2: Stmt)
+        | If(cond: Expr, t: Stmt, f: Stmt)
+
+    // Runtime model
+    
+    // We model the concrete environment as a map with variable names as the keys to their corresponding values as the value.
+    // If a variable is missing from the map, it is "uninitialized", and it will cause an error if it is accessed (without having been initialized).
+    type Env = map<string, int>
+
+    // Runtime errors to detect for.
+    datatype RuntimeError =
+        | DivByZero
+        | UninitializedVar(x: string)
+        // out of bounds
+
+    // Result can either be Ok, or a runtime error.
+    datatype Result<T> =
+        | Ok(v: T)
+        | Err(e: RuntimeError)
+
+    // Set/Update a variable
+    function Update(env: Env, x: string, v: int): Env
+        ensures x in Update(env, x, v)
+        ensures Update(env, x, v)[x] == v
+    {
+        env[x := v]
+    }
+}
