README.md
@@ -1,2 +1,44 @@
 # Static-Analyzer
 Static Analyzer, final project for ECS 261
+
+## Getting started.
+Verify the files
+
+```bash
+dafny verify Types.dfy StaticAnalyzer.dfy Tests.dfy
+```
+
+## Add your own test cases/programs.
+Create your own dafny test file, you can copy the starter code below.
+
+```dafny
+include "Types.dfy" 
+include "StaticAnalyzer.dfy" 
+
+module Tests{
+    import opened StaticAnalyzer
+    import opened Types
+
+    // write tests here
+}
+```
+
+```dafny
+    method TestCaseNAME(){
+        /*
+        Put the readable syntax version of your program here.
+        */
+        var stmt := // Fill this in. default is "Skip()"
+        var env := // Fill this in. default is "map[];"
+
+        var safe := AnalyzeProgram(stmt, env);
+        assert safe; // or !safe if your prog is potentially erroneous, dafny will give an error.
+        AnalyzeProgramSound(stmt, env);
+
+        match ExecStmt(stmt, env)
+        case Ok(envOut) => assert // this will have either Ok(envOut) or false, you can verify the value here
+        case Err(e) => assert // this will have either a Err(RuntimeError) or false, you can verify the error type here
+    }
+```
+
+Reference Types.dfy for the types of statements/expressions and Tests.py for examples.
